link.v
@@ -124,7 +124,7 @@ Section Link_Template.
   (* The node-level invariant (γ in the paper).
    * See also link.spl for the matching GRASShopper definition *)
   Definition nodeinv I_n n: Prop :=
-    (∀ k, k ∈ linkset I_n n ∧ ¬ in_outsets k I_n → in_inset k I_n n).    
+    (∀ k, k ∈ linkset K I_n n ∧ ¬ in_outsets K k I_n → in_inset K k I_n n).    
 
   (* The following hypothesis is proved as GRASShopper lemmas in 
    * hashtbl-link.spl and b-link.spl *)
@@ -154,72 +154,78 @@ Section Link_Template.
   (* The following functions are proved for each implementation in GRASShopper
    * (see b-link.spl and hashtbl-link.spl *)
 
+  (* Todo: Can we simplify the match to ⌜b → in_inset k I_n n⌝? *)
   Parameter findNext_spec : ∀ (n: Node) (I_n : linkset_flowint_ur K) (C: gset K) (k: K),
-    ({{{ node n I_n C ∗ ⌜k ∈ linkset I_n n ∨ in_inset k I_n n⌝ }}}
+    ({{{ node n I_n C ∗ ⌜k ∈ linkset K I_n n ∨ in_inset K k I_n n⌝ }}}
       findNext #n #k
     {{{ (b: bool) (n': Node), 
         RET (match b with true => (SOMEV #n') | false => NONEV end); 
-        node n I_n C ∗ (match b with true => ⌜in_outset k I_n n'⌝ |
-                                    false => ⌜¬in_outsets k I_n⌝ end) }}})%I.
+        node n I_n C ∗ (match b with true => ⌜in_outset K k I_n n'⌝ |
+                                    false => ⌜¬in_outsets K k I_n⌝ end) }}})%I.
 
-  Parameter decisiveOp_spec : ∀ (dop: dOp) (n: Node) (k: K) (I_n: linkset_flowint_ur K) (C: gset K),
-    ({{{ node n I_n C ∗ ⌜in_inset k I_n n⌝ ∗ ⌜¬in_outsets k I_n⌝ }}}
+  Parameter decisiveOp_spec : ∀ (dop: dOp) (n: Node) (k: K)
+      (I_n: linkset_flowint_ur K) (C: gset K),
+    ({{{ node n I_n C ∗ ⌜in_inset K k I_n n⌝ ∗ ⌜¬in_outsets K k I_n⌝ }}}
       decisiveOp dop #n #k
     {{{ (b: bool) (C': gset K) (res: bool),
         RET (match b with false => NONEV | true => (SOMEV #res) end);
         match b with false => node n I_n C |
-                      true => node n I_n C' ∗ Ψ dop k C C' res ∗ ⌜ C' ⊆ keyset I_n n⌝
+                      true => node n I_n C' ∗ Ψ dop k C C' res
+                              ∗ ⌜ C' ⊆ keyset K I_n n⌝
         end }}})%I.
 
-  (* ---------- The invariant ---------- *)
-  
-  Definition CCS γ γ_fp γ_k γ_inr γ_fi root I C : iProp :=                             
-    (own γ (● I) ∗ own γ_k (● prod (KS, C)) ∗ own γ_fp (● dom I) ∗ ⌜globalinv root I⌝
-    ∗ ([∗ set] n ∈ (dom I), (∃ (b: bool) (I_n: linkset_flowint_ur K),
+  (** The concurrent search structure invariant *)
+
+  Definition CCS γ γ_fp γ_k γ_inr γ_fi root I C : iProp :=
+    (own γ (● I) ∗ own γ_k (● prod (KS, C)) ∗ own γ_fp (● domm I) ∗ ⌜globalinv K root I⌝
+    ∗ ([∗ set] n ∈ (domm I), (∃ (b: bool) (I_n: linkset_flowint_ur K),
       (lockLoc n) ↦ #b
       ∗ (if b then True
-        else (∃ C_n, node n I_n C_n ∗ own (γ_fi n) ((●{1/2} I_n)) ∗ own γ_k (◯ prod (keyset I_n n, C_n))))
-      ∗ own γ (◯ I_n) ∗ ⌜dom I_n = {[n]}⌝ ∗ own (γ_fi n) ((●{1/2} I_n))
-      ∗ own (γ_inr n) (● (linkset I_n n))))
+        else (∃ C_n, node n I_n C_n ∗ own (γ_fi n) ((●{1/2} I_n)) ∗ own γ_k (◯ prod (keyset K I_n n, C_n))))
+      ∗ own γ (◯ I_n) ∗ ⌜domm I_n = {[n]}⌝ ∗ own (γ_fi n) ((●{1/2} I_n))
+      ∗ own (γ_inr n) (● (linkset K I_n n))))
     )%I.    
 
-  Definition is_CCS γ γ_fp γ_k γ_inr γ_fi root C := (∃ I, (CCS γ γ_fp γ_k γ_inr γ_fi root I C))%I.
+  Definition is_CCS γ γ_fp γ_k γ_inr γ_fi root C :=
+    (∃ I, (CCS γ γ_fp γ_k γ_inr γ_fi root I C))%I.
 
-  (* ---------- Assorted useful lemmas ---------- *)
+  (** Assorted useful lemmas *)
 
-  Lemma globalinv_root_fp: ∀ I root, globalinv root I → root ∈ dom I.
+  Lemma globalinv_root_fp: ∀ I root, globalinv K root I → root ∈ domm I.
   Proof. 
     intros I root Hglob. unfold globalinv in Hglob.
     destruct Hglob as [H1 [H2 H3]]. done.
   Qed.
 
   Lemma globalinv_root_inr : ∀ I Ir root k,
-    globalinv root I ∧ Ir ≼ I ∧ dom Ir = {[root]} → k ∈ linkset Ir root.
+    globalinv K root I ∧ Ir ≼ I ∧ domm Ir = {[root]} → k ∈ linkset K Ir root.
   Proof.
-    intros I Ir root k Hglob. destruct Hglob as [Hglob [H1 H2]].
-    unfold globalinv in Hglob. destruct Hglob as [H3 [H4 [H5 H6]]].
-    specialize (H6 root). assert (k ∈ linkset I root).
-    { apply H6. done. } destruct H1 as [I2 H1].
-     apply (linkset_monotone I Ir I2 k root); try done. set_solver.
-  Qed. 
+    intros I Ir root k ((Hv & _ & _ & H6 & _) & [I2 Hincl] & Hdom).
+    apply (linkset_monotone I Ir I2 k root); try done.
+    apply H6.
+    set_solver.
+  Qed.
 
-  Lemma auth_own_incl γ (x y: linkset_flowint_ur K) : own γ (● x) ∗ own γ (◯ y) -∗ ⌜y ≼ x⌝.
+  Lemma auth_set_incl {A: Type} `{Countable A} `{inG Σ (authR (gsetUR A))}
+      (γ_fp: gname) (Ns Ns': gset A) :
+    own γ_fp (◯ Ns) ∗ own γ_fp (● Ns') -∗ ⌜Ns ⊆ Ns'⌝.
+  Proof.
+    rewrite -own_op. rewrite own_valid. iPureIntro.
+    rewrite auth_valid_discrete. simpl. rewrite ucmra_unit_right_id_L.
+    intros (_ & [a (Hagree & Hincl & _)]).
+    apply gset_included in Hincl.
+    apply to_agree_inj in Hagree. set_solver.
+  Qed.
+
+  Lemma auth_own_incl γ (x y: linkset_flowint_ur K) :
+    own γ (● x) ∗ own γ (◯ y) -∗ ⌜y ≼ x⌝.
   Proof.
     rewrite -own_op. rewrite own_valid. iPureIntro.
     apply auth_both_valid.
   Qed.
 
-  Lemma auth_set_incl γ_fp Ns Ns' :
-    own γ_fp (◯ Ns) ∗ own γ_fp (● Ns') -∗ ⌜Ns ⊆ Ns'⌝.
-  Proof.
-    rewrite -own_op. rewrite own_valid. iPureIntro.
-    rewrite auth_valid_discrete. simpl. rewrite ucmra_unit_right_id_L.
-    intros. destruct H. inversion H0 as [m H1].
-    destruct H1. destruct H2. apply gset_included in H2.
-    apply to_agree_inj in H1. set_solver.
-  Qed.  
-
-  Lemma auth_own_incl_ks γ (x y: keysetUR) : own γ (● x) ∗ own γ (◯ y) -∗ ⌜y ≼ x⌝.
+  Lemma auth_own_incl_ks γ (x y: keysetUR K) :
+    own γ (● x) ∗ own γ (◯ y) -∗ ⌜y ≼ x⌝.
   Proof.
     rewrite -own_op. rewrite own_valid. iPureIntro. rewrite auth_valid_discrete.
     simpl. intros H. destruct H. destruct H0 as [a Ha]. destruct Ha as [Ha Hb].
@@ -229,12 +235,13 @@ Section Link_Template.
     rewrite Hy in Hb. rewrite <- Ha in Hb. done.
   Qed.
 
-  (* ---------- Lock module proofs ---------- *)
 
-  Lemma lockNode_spec (n: Node):
+  (** Lock module proofs *)
+
+  Lemma lockNode_spec (n: Node): (* TODO rewrite if then else *)
     <<< ∀ (b: bool), (lockLoc n) ↦ #b >>>
       lockNode #n    @ ⊤
-    <<< (lockLoc n) ↦ #true ∗ if b then False else True, RET #() >>>. (* rewrite if then else *)
+    <<< (lockLoc n) ↦ #true ∗ if b then False else True, RET #() >>>.
   Proof.
     iIntros (Φ) "AU". iLöb as "IH".
     wp_lam. wp_bind(getLockLoc _)%E.
@@ -268,6 +275,120 @@ Section Link_Template.
     iMod ("Hclose" with "Hy") as "HΦ".
     iModIntro. done.
   Qed.
+
+  
+  (** Proofs of traverse and CCSOp *)
+
+  Lemma traverse_spec (γ γ_fp γ_k: gname) (γ_inr γ_fi: Node → gname)
+      (root: Node) (k: K) (n: Node) (Ns: gset Node) (I_n:linkset_flowint_ur K):
+    ⌜n ∈ Ns⌝ ∗ own γ_fp (◯ Ns)
+    ∗ own (γ_inr n) (◯ (linkset K I_n n)) ∗ ⌜k ∈ linkset K I_n n⌝ -∗ 
+    <<< ∀ C, is_CCS γ γ_fp γ_k γ_inr γ_fi root C >>>
+      traverse #n #k @ ⊤
+    <<< ∃ (n': Node) (Ns': gsetUR Node) (I_n': linkset_flowint_ur K) (Cn': gset K),
+        is_CCS γ γ_fp γ_k γ_inr γ_fi root C ∗ ⌜n' ∈ Ns'⌝
+        ∗ own γ_fp (◯ Ns') ∗ node n' I_n' Cn' ∗ own (γ_fi n') ((●{1/2} I_n'))
+        ∗ own γ_k (◯ prod (keyset K I_n' n', Cn')) ∗ ⌜domm I_n' = {[n']}⌝
+        ∗ ⌜in_inset K k I_n' n'⌝ ∗ ⌜¬in_outsets K k I_n'⌝, RET #n' >>>.
+  Proof.
+    iLöb as "IH" forall (n Ns I_n). iIntros "(#Hinn & #Hfp & #Hinrfp & #Hkinr)".
+    iDestruct "Hinn" as %Hinn.
+    iIntros (Φ) "AU". wp_lam. wp_let. wp_bind(lockNode _)%E.
+    awp_apply (lockNode_spec n). iApply (aacc_aupd_abort with "AU"); first done.
+    iIntros (C0) "Hst". iDestruct "Hst" as (I) "(HI & HKS & HNDS & Hglob & Hstar)".
+    iAssert (⌜n ∈ domm I⌝)%I with "[HNDS]" as "%".
+    { iPoseProof ((auth_set_incl γ_fp Ns (domm I)) with "[$]") as "%".
+      iPureIntro. set_solver. }
+    rewrite (big_sepS_elem_of_acc _ (domm I) n); last by eauto.
+    iDestruct "Hstar" as "[Hn Hstar]".
+    iDestruct "Hn" as (b In) "(Hlock & Hb & HIn & #HNds & Hfis & Hks)".
+    iAaccIntro with "Hlock". { iIntros "H". iModIntro. iSplitL. iFrame "∗ % #".
+    iExists I. iFrame "∗ % #". iApply "Hstar". iExists b, In.
+    iFrame "# % ∗". eauto with iFrame. } iIntros "(Hloc & ?)".
+    destruct b. { iExFalso. done. } iModIntro.
+    iPoseProof ((auth_set_incl (γ_inr n)) with "[$Hks $Hinrfp]") as "%".
+    iDestruct "Hkinr" as "%". assert (k ∈ linkset K In n) as Hkinr. { set_solver. }
+    iPoseProof (own_valid with "HIn") as "%". rename H2 into HInV.
+    assert (✓ In) as HInv. { apply (auth_frag_valid (◯ In)). done. }
+    iSplitR "Hb". iFrame "∗ % #". iExists I. iFrame "∗ % #". iApply "Hstar". iExists true, In.
+    iFrame "# % ∗". iIntros "AU". iModIntro. wp_pures.
+    iDestruct "Hb" as (Cn) "(Hrep & Hfil & Hks)". iDestruct "HNds" as %HNds.
+    wp_bind (findNext _ _)%E. wp_apply ((findNext_spec n In Cn k) with "[Hrep]").
+    iFrame; iPureIntro; left; done. iIntros (b n') "(Hrep & Hb)". destruct b. 
+    - wp_pures. awp_apply (unlockNode_spec n). 
+      iApply (aacc_aupd_abort with "AU"); first done. iIntros (C1) "Hst".
+      iDestruct "Hst" as (I1) "(HI & HKS & HNDS & Hglob & Hstar)".
+      iAssert (⌜n ∈ domm I1⌝)%I with "[HNDS]" as "%".
+      { iPoseProof ((auth_set_incl γ_fp Ns (domm I1)) with "[$]") as "%".
+        iPureIntro. set_solver. }
+      rewrite (big_sepS_delete _ (domm I1) n); last by eauto. iDestruct "Hstar" as "(Hcln & Hstar)".
+      iDestruct "Hcln" as (b In1) "(Hlock & Hbb & HIn & #HNds1 & Hfis & Hks1)".
+      destruct b; first last. { iDestruct "Hbb" as (Cn') "(Hrep' & _)".
+      iAssert (⌜False⌝)%I with "[Hrep Hrep']" as %Hf. { iApply (node_sep_star n In In1). 
+      iFrame. } exfalso. done. }
+      iPoseProof ((own_valid_2 (γ_fi n) (●{1 / 2} In) (●{1 / 2} In1)) with "[Hfil] [Hfis]") as "%"; try done.
+      apply (auth_auth_frac_op_inv _ _ _ _) in H3. apply leibniz_equiv in H3. replace In1.            
+      iDestruct "Hb" as %Hb. iDestruct "HNds1" as %HNds1. iDestruct "Hglob" as %Hglob.
+      iPoseProof (auth_own_incl with "[$HI $HIn]") as (I2)"%".
+      iPoseProof (own_valid with "HI") as "%". iAssert (⌜n' ∈ domm I1⌝)%I as "%".
+      { iPureIntro. assert (n' ∈ domm I2).
+        { apply (flowint_step I1 In I2 k n' root); try done. }
+        assert (domm I1 = domm In ∪ domm I2).
+        { rewrite H4. apply flowint_comp_fp. 
+          rewrite H4 in H5 * => H5.
+          rewrite <-H4.
+          apply auth_auth_valid.
+          rewrite <-H4 in H5. done.
+        }
+        rewrite H7.
+        set_solver. }
+      (* apply Hglob. } *)
+      assert (n ≠ n') as Hneq.
+      { assert (n' ∉ domm In).
+        { apply (outset_distinct In n').
+          split. done.
+          exists k. done. }
+        rewrite HNds1 in H7. set_solver. }
+      rewrite (big_sepS_delete _ (domm I1 ∖ {[n]}) n'); last first.
+      set_solver. iDestruct "Hstar" as "(Hcln' & Hstar)". 
+      iDestruct "Hcln'" as (b In') "(Hlock' & Hbb' & HIn' & #HNds' & Hfis' & Hks1')".
+      iPoseProof ((own_op γ (◯ In) (◯ In' )) with "[HIn HIn']") as "H"; first by eauto with iFrame.
+      iPoseProof (own_valid with "H") as "%". rewrite -auth_frag_op in H7.
+      assert (✓ (In ⋅ In')). { apply (auth_frag_valid (◯ (In ⋅ In'))). done. }
+      iDestruct "HNds'" as %HNds'. assert (k ∈ linkset K In' n').
+      {
+        admit.
+        (* TODO need to adapt proof to new version of flowint_linkset_step.
+           I think one issue is that this proof assumes linkset is a superset
+           of inset, whereas the formulation in linkset_flows.v does not.
+           So maybe even the traverse spec might have to be updated. *)
+        (* apply (flowint_linkset_step (In⋅In') In In' k n n'); try done. *)
+      }
+      assert (root ∈ domm I1). { apply globalinv_root_fp. done. } iDestruct "H" as "(HIn & HIn')".
+      iMod (own_update (γ_inr n') (● linkset K In' n') (● linkset K In' n' ⋅ ◯ linkset K In' n') with "Hks1'") as "HNs".
+      apply auth_update_core_id. apply gset_core_id. done. iDestruct "HNs" as "(Hks1' & #Hinr1')".
+      iAaccIntro with "Hlock". { iIntros "Hlock". iModIntro. iSplitR "Hfil Hks Hrep". iFrame "∗ # %".
+      iExists I1. iFrame "∗ % #". rewrite (big_sepS_delete _ (domm I1) n); last by eauto.
+      iSplitR "Hstar Hbb' HIn' Hfis' Hks1' Hlock'". iExists true, In. iFrame "# % ∗".
+      rewrite (big_sepS_delete _ (domm I1 ∖ {[n]}) n'); last first. set_solver. iFrame. iExists b, In'.
+      iFrame "# % ∗".  iIntros "AU". iModIntro. iFrame "# % ∗". } iIntros "Hlock".
+      iMod (own_update γ_fp (● domm I1) (● domm I1 ⋅ ◯ domm I1) with "HNDS") as "HNs".
+      apply auth_update_core_id. apply gset_core_id. done. iDestruct "HNs" as "(HAfp & #Hfp1)".
+      iModIntro. iSplitL. iExists I1. iFrame "∗ % #". rewrite (big_sepS_delete _ (domm I1) n); last by eauto.
+      iSplitR "Hstar Hbb' HIn' Hfis' Hks1' Hlock'". iExists false, In. iFrame "# % ∗". iExists Cn. iFrame.
+      rewrite (big_sepS_delete _ (domm I1 ∖ {[n]}) n'); last first. set_solver. iFrame. iExists b, In'.
+      iFrame "# % ∗". iIntros "AU". iModIntro. wp_pures. iSpecialize ("IH" $! n' (domm I1) In').
+      iApply "IH". iFrame "∗ # %". done.
+    - iApply fupd_wp. iMod "AU" as (C) "[Hst [_ Hclose]]". iSpecialize ("Hclose" $! n Ns In Cn).
+      iMod ("Hclose" with "[Hst Hfil Hks Hrep Hb]") as "HΦ". iDestruct "Hb" as %Hnotout.
+      iAssert (node n In Cn ∗ ⌜nodeinv In n⌝)%I with "[Hrep]" as "(Hrep & Hninv)".
+      { iApply (node_implies_nodeinv _ _ _). iFrame "∗ # %". } iDestruct "Hninv" as %Hninv.
+      iFrame "∗ # %". iPureIntro. unfold nodeinv in Hninv. specialize (Hninv k).
+      apply Hninv. try done. iModIntro. wp_pures. done.
+  Admitted.
+
+
+  (* Ghost state manipulation to make final proof cleaner *)
 
   (* Todo: I think k ∈ KS follows from k ∈ K1, so we can drop it here,
     and in CCSOp_spec. *)
@@ -330,93 +451,6 @@ Section Link_Template.
 
   (* ---------- Proofs of traverse and CCSOp ---------- *)
 
-  Lemma traverse_spec (γ γ_fp γ_k: gname) γ_inr γ_fi root (k: K) (n: Node) (Ns: gset Node) (I_n:linkset_flowint_ur K) :
-    ⌜n ∈ Ns⌝ ∗ own γ_fp (◯ Ns)
-    ∗ own (γ_inr n) (◯ (linkset I_n n)) ∗ ⌜k ∈ linkset I_n n⌝ -∗ 
-    <<< ∀ C, is_CCS γ γ_fp γ_k γ_inr γ_fi root C >>>
-      traverse #n #k @ ⊤
-    <<< ∃ (n': Node) (Ns': gsetUR Node) (I_n': linkset_flowint_ur K) (Cn': gset K),
-        is_CCS γ γ_fp γ_k γ_inr γ_fi root C ∗ ⌜n' ∈ Ns'⌝
-        ∗ own γ_fp (◯ Ns') ∗ node n' I_n' Cn' ∗ own (γ_fi n') ((●{1/2} I_n'))
-        ∗ own γ_k (◯ prod (keyset I_n' n', Cn')) ∗ ⌜dom I_n' = {[n']}⌝
-        ∗ ⌜in_inset k I_n' n'⌝ ∗ ⌜¬in_outsets k I_n'⌝, RET #n' >>>.
-  Proof.
-    iLöb as "IH" forall (n Ns I_n). iIntros "(#Hinn & #Hfp & #Hinrfp & #Hkinr)".
-    iDestruct "Hinn" as %Hinn.
-    iIntros (Φ) "AU". wp_lam. wp_let. wp_bind(lockNode _)%E.
-    awp_apply (lockNode_spec n). iApply (aacc_aupd_abort with "AU"); first done.
-    iIntros (C0) "Hst". iDestruct "Hst" as (I) "(HI & HKS & HNDS & Hglob & Hstar)".
-    iAssert (⌜n ∈ dom I⌝)%I with "[HNDS]" as "%".
-    { iPoseProof ((auth_set_incl γ_fp Ns (dom I)) with "[$]") as "%".
-      iPureIntro. set_solver. }
-    rewrite (big_sepS_elem_of_acc _ (dom I) n); last by eauto.
-    iDestruct "Hstar" as "[Hn Hstar]".
-    iDestruct "Hn" as (b In) "(Hlock & Hb & HIn & #HNds & Hfis & Hks)".
-    iAaccIntro with "Hlock". { iIntros "H". iModIntro. iSplitL. iFrame "∗ % #".
-    iExists I. iFrame "∗ % #". iApply "Hstar". iExists b, In.
-    iFrame "# % ∗". eauto with iFrame. } iIntros "(Hloc & ?)".
-    destruct b. { iExFalso. done. } iModIntro. 
-    iPoseProof (auth_set_incl with "[$Hks $Hinrfp]") as "%".
-    iDestruct "Hkinr" as "%". assert (k ∈ linkset In n) as Hkinr. { set_solver. }
-    iPoseProof (own_valid with "HIn") as "%". rename H2 into HInV.
-    assert (✓ In) as HInv. { apply (auth_frag_valid (◯ In)). done. }
-    iSplitR "Hb". iFrame "∗ % #". iExists I. iFrame "∗ % #". iApply "Hstar". iExists true, In.
-    iFrame "# % ∗". iIntros "AU". iModIntro. wp_pures.
-    iDestruct "Hb" as (Cn) "(Hrep & Hfil & Hks)". iDestruct "HNds" as %HNds.
-    wp_bind (findNext _ _)%E. wp_apply ((findNext_spec n In Cn k) with "[Hrep]").
-    iFrame; iPureIntro; left; done. iIntros (b n') "(Hrep & Hb)". destruct b. 
-    - wp_pures. awp_apply (unlockNode_spec n). 
-      iApply (aacc_aupd_abort with "AU"); first done. iIntros (C1) "Hst".
-      iDestruct "Hst" as (I1) "(HI & HKS & HNDS & Hglob & Hstar)".
-      iAssert (⌜n ∈ dom I1⌝)%I with "[HNDS]" as "%".
-      { iPoseProof ((auth_set_incl γ_fp Ns (dom I1)) with "[$]") as "%".
-        iPureIntro. set_solver. }
-      rewrite (big_sepS_delete _ (dom I1) n); last by eauto. iDestruct "Hstar" as "(Hcln & Hstar)".
-      iDestruct "Hcln" as (b In1) "(Hlock & Hbb & HIn & #HNds1 & Hfis & Hks1)".
-      destruct b; first last. { iDestruct "Hbb" as (Cn') "(Hrep' & _)".
-      iAssert (⌜False⌝)%I with "[Hrep Hrep']" as %Hf. { iApply (node_sep_star n In In1). 
-      iFrame. } exfalso. done. }
-      iPoseProof ((own_valid_2 (γ_fi n) (●{1 / 2} In) (●{1 / 2} In1)) with "[Hfil] [Hfis]") as "%"; try done.
-      apply (auth_auth_frac_op_inv _ _ _ _) in H3. apply leibniz_equiv in H3. replace In1.            
-      iDestruct "Hb" as %Hb. iDestruct "HNds1" as %HNds1. iDestruct "Hglob" as %Hglob.
-      iPoseProof (auth_own_incl with "[$HI $HIn]") as (I2)"%".
-      iPoseProof (own_valid with "HI") as "%". iAssert (⌜n' ∈ dom I1⌝)%I as "%".
-      { iPureIntro. assert (n' ∈ dom I2). { apply (flowint_step I1 In I2 k n' root). done. 
-        apply auth_auth_valid. done. done. done. }
-        apply flowint_comp_fp in H4. set_solver. apply Hglob. }
-      assert (n ≠ n') as Hneq. { assert (n' ∉ dom In). { apply (outset_distinct In n').
-      exists k. done. } rewrite HNds1 in H7. set_solver. }
-      rewrite (big_sepS_delete _ (dom I1 ∖ {[n]}) n'); last first.
-      set_solver. iDestruct "Hstar" as "(Hcln' & Hstar)". 
-      iDestruct "Hcln'" as (b In') "(Hlock' & Hbb' & HIn' & #HNds' & Hfis' & Hks1')".
-      iPoseProof ((own_op γ (◯ In) (◯ In' )) with "[HIn HIn']") as "H"; first by eauto with iFrame.
-      iPoseProof (own_valid with "H") as "%". rewrite -auth_frag_op in H7.
-      assert (✓ (In ⋅ In')). { apply (auth_frag_valid (◯ (In ⋅ In'))). done. }
-      iDestruct "HNds'" as %HNds'. assert (k ∈ linkset In' n').
-      { apply (flowint_linkset_step (In⋅In') In In' k n n'); try done. }
-      assert (root ∈ dom I1). { apply globalinv_root_fp. done. } iDestruct "H" as "(HIn & HIn')".
-      iMod (own_update (γ_inr n') (● linkset In' n') (● linkset In' n' ⋅ ◯ linkset In' n') with "Hks1'") as "HNs".
-      apply auth_update_core_id. apply gset_core_id. done. iDestruct "HNs" as "(Hks1' & #Hinr1')".
-      iAaccIntro with "Hlock". { iIntros "Hlock". iModIntro. iSplitR "Hfil Hks Hrep". iFrame "∗ # %".
-      iExists I1. iFrame "∗ % #". rewrite (big_sepS_delete _ (dom I1) n); last by eauto.
-      iSplitR "Hstar Hbb' HIn' Hfis' Hks1' Hlock'". iExists true, In. iFrame "# % ∗". 
-      rewrite (big_sepS_delete _ (dom I1 ∖ {[n]}) n'); last first. set_solver. iFrame. iExists b, In'.
-      iFrame "# % ∗".  iIntros "AU". iModIntro. iFrame "# % ∗". } iIntros "Hlock".
-      iMod (own_update γ_fp (● dom I1) (● dom I1 ⋅ ◯ dom I1) with "HNDS") as "HNs".
-      apply auth_update_core_id. apply gset_core_id. done. iDestruct "HNs" as "(HAfp & #Hfp1)".
-      iModIntro. iSplitL. iExists I1. iFrame "∗ % #". rewrite (big_sepS_delete _ (dom I1) n); last by eauto.
-      iSplitR "Hstar Hbb' HIn' Hfis' Hks1' Hlock'". iExists false, In. iFrame "# % ∗". iExists Cn. iFrame. 
-      rewrite (big_sepS_delete _ (dom I1 ∖ {[n]}) n'); last first. set_solver. iFrame. iExists b, In'.
-      iFrame "# % ∗". iIntros "AU". iModIntro. wp_pures. iSpecialize ("IH" $! n' (dom I1) In').
-      iApply "IH". iFrame "∗ # %". done.
-    - iApply fupd_wp. iMod "AU" as (C) "[Hst [_ Hclose]]". iSpecialize ("Hclose" $! n Ns In Cn).
-      iMod ("Hclose" with "[Hst Hfil Hks Hrep Hb]") as "HΦ". iDestruct "Hb" as %Hnotout.
-      iAssert (node n In Cn ∗ ⌜nodeinv In n⌝)%I with "[Hrep]" as "(Hrep & Hninv)". 
-      { iApply (node_implies_nodeinv _ _ _). iFrame "∗ # %". } iDestruct "Hninv" as %Hninv. 
-      iFrame "∗ # %". iPureIntro. unfold nodeinv in Hninv. specialize (Hninv k).
-      apply Hninv. try done. iModIntro. wp_pures. done.
-  Qed.
-
   Theorem CCSOp_spec (γ γ_fp γ_k: gname) γ_inr γ_fi root (k: K) (dop: dOp):
     ⌜k ∈ KS⌝ -∗ <<< ∀ C, is_CCS γ γ_fp γ_k γ_inr γ_fi root C >>>
       CCSOp dop root #k @ ⊤
@@ -427,21 +461,21 @@ Section Link_Template.
     iApply fupd_wp. iMod "AU" as (C0) "[Hst [HAU _]]".
     iDestruct "Hst" as (I0) "(HI & HKS & HNDS & #Hglob & Hstar)".
     iDestruct "Hglob" as %Hglob. iDestruct "HKin" as %HKin. 
-    assert (root ∈ dom I0)%I as Hroot. { apply globalinv_root_fp. done. }
-    iMod (own_update γ_fp (● dom I0) (● dom I0 ⋅ ◯ dom I0) with "HNDS") as "H".
+    assert (root ∈ domm I0)%I as Hroot. { apply globalinv_root_fp. done. }
+    iMod (own_update γ_fp (● domm I0) (● domm I0 ⋅ ◯ domm I0) with "HNDS") as "H".
     { apply auth_update_core_id. apply gset_core_id. done. } 
     iDestruct "H" as "(HNDS & #Hfp0)".
-    rewrite (big_sepS_elem_of_acc _ (dom I0) root); last by eauto.
+    rewrite (big_sepS_elem_of_acc _ (domm I0) root); last by eauto.
     iDestruct "Hstar" as "[Hn Hstar]".
     iDestruct "Hn" as (b Ir) "(H1 & H2 & H3 & H4 & H5 & Hksr)".
     iPoseProof (auth_own_incl with "[$HI $H3]") as "%". iDestruct "H4" as %HNdsr.
     (*assert (inreach Ir root = inreach I0 root) as Hinreach. { apply globalinv_inreach; try done. }*)
-    iMod (own_update (γ_inr root) (● linkset Ir root) (● linkset Ir root ⋅ ◯ linkset Ir root) with "Hksr") as "H".
+    iMod (own_update (γ_inr root) (● linkset K Ir root) (● linkset K Ir root ⋅ ◯ linkset K Ir root) with "Hksr") as "H".
     apply auth_update_core_id. apply gset_core_id. done. iDestruct "H" as "(Hksr & #Hinr)".
     iMod ("HAU" with "[HI HKS H1 H2 H3 H5 Hstar HNDS Hksr] ") as "AU". 
     { iExists I0. iFrame "∗ % #". iApply "Hstar". iExists b, Ir. iFrame "∗ # %". }
     iModIntro. wp_bind (traverse _ _)%E.
-    awp_apply (traverse_spec γ γ_fp γ_k γ_inr γ_fi root k root (dom I0) Ir). iFrame "∗ # %".
+    awp_apply (traverse_spec γ γ_fp γ_k γ_inr γ_fi root k root (domm I0) Ir). iFrame "∗ # %".
     iPureIntro. apply (globalinv_root_inr I0 Ir root k); try done.
     iApply (aacc_aupd_abort with "AU"); first done.
     iIntros (C1) "Hst". iAaccIntro with "Hst"; first by eauto with iFrame.
@@ -456,10 +490,10 @@ Section Link_Template.
       iApply (aacc_aupd_commit with "AU"); first done. iIntros (C2) "Hst".
       iDestruct "Hst" as (I) "(HI & HKS & HNDS & #Hglob & Hstar)". 
       iDestruct "Hglob" as %Hglob'.
-      iAssert (⌜n ∈ dom I⌝)%I with "[HNDS]" as "%".
-      { iPoseProof ((auth_set_incl γ_fp Ns (dom I)) with "[$]") as "%".
+      iAssert (⌜n ∈ domm I⌝)%I with "[HNDS]" as "%".
+      { iPoseProof ((auth_set_incl γ_fp Ns (domm I)) with "[$]") as "%".
       iPureIntro. set_solver. }
-      rewrite (big_sepS_elem_of_acc _ (dom I) n); last by eauto.
+      rewrite (big_sepS_elem_of_acc _ (domm I) n); last by eauto.
       iDestruct "Hstar" as "[Hn Hstar]".
       iDestruct "Hn" as (b' In1) "(Hlock & Hb & HIn & #HNds & Hfis & Hinreach)".
       destruct b'; first last. { iDestruct "Hb" as (Cn'') "(Hrep' & _)".
@@ -476,7 +510,7 @@ Section Link_Template.
       assert (✓ In) as HInv. { apply (auth_frag_valid (◯ In)). done. }
       iAssert (node n In Cn' ∗ ⌜nodeinv In n⌝)%I with "[Hrep]" as "(Hrep & Hninv)". 
       { iApply (node_implies_nodeinv _ _ _). iFrame "% ∗ #". } iDestruct "Hninv" as %Hninv.                   
-      iMod ((ghost_update_keyset γ_k dop k Cn Cn' res (keyset In n) C2) with "[HKS Hks]") as "Hgks".
+      iMod ((ghost_update_keyset γ_k dop k Cn Cn' res (keyset K In n) C2) with "[HKS Hks]") as "Hgks".
       iFrame "% ∗ #". iPureIntro. apply keyset_def; try done.
       iDestruct "Hgks" as (C2') "(#HΨC & Ha & Hf)".
       iModIntro. iExists (C2'), res. iSplitL. iSplitR "HΨC".
@@ -488,10 +522,10 @@ Section Link_Template.
       iApply (aacc_aupd_abort with "AU"); first done. iIntros (C2) "Hst".
       iDestruct "Hst" as (I) "(HI & HKS & HNDS & #Hglob & Hstar)". 
       iDestruct "Hglob" as %Hglob'.
-      iAssert (⌜n ∈ dom I⌝)%I with "[HNDS]" as "%".
-      { iPoseProof ((auth_set_incl γ_fp Ns (dom I)) with "[$]") as "%".
+      iAssert (⌜n ∈ domm I⌝)%I with "[HNDS]" as "%".
+      { iPoseProof ((auth_set_incl γ_fp Ns (domm I)) with "[$]") as "%".
       iPureIntro. set_solver. }
-      rewrite (big_sepS_elem_of_acc _ (dom I) n); last by eauto.
+      rewrite (big_sepS_elem_of_acc _ (domm I) n); last by eauto.
       iDestruct "Hstar" as "[Hn Hstar]".
       iDestruct "Hn" as (b' In1) "(Hlock & Hb' & HIn & #HNds & Hfis & Hinreach)".
       destruct b'; first last. { iDestruct "Hb'" as (Cn'') "(Hrep' & _)".
